Shows status as of 5th Sept

i2c/i2cCircuitScript.sml
@@ -1,7 +1,7 @@
 open HolKernel Parse boolLib bossLib;
 open wordsTheory;
 open translatorLib;
-open i2cRegsCircuitLib i2cCoreCircuitLib;
+open i2cRegsCircuitLib;
 open cheshireCircuitTheory i2cCircuitStateTheory;
 
 val _ = new_theory "i2cCircuit";
@@ -22,363 +22,644 @@ Theorem i2c_reg_top_comb_1_trans = SIMP_RULE (pure_ss ++ ARITH_ss) [reg_req_deco
 
 (* Section --- I2C Core *)
 
+Overload idle = “0w : 5 word”;
+Overload active = “1w : 5 word”;
+Overload recReadClockLow = “2w : 5 word”;
+Overload recReadClockPulse = “3w : 5 word”;
+Overload recReadHoldBit = “4w : 5 word”;
+Overload recHostClockLowAck = “5w : 5 word”;
+Overload recHostClockPulseAck = “6w : 5 word”;
+Overload recHostHoldBitAck = “7w : 5 word”;
+Overload stopClockStop = “8w : 5 word”;
+Overload stopSetupStop = “9w : 5 word”;
+Overload stopHoldStop = “10w : 5 word”;
+Overload startSetupStart = “11w : 5 word”;
+Overload startHoldStart = “12w : 5 word”;
+Overload startClockStart = “13w : 5 word”;
+Overload transClockLow = “14w : 5 word”;
+Overload transClockPulse = “15w : 5 word”;
+Overload transHoldBit = “16w : 5 word”;
+Overload transClockLowAck = “17w : 5 word”;
+Overload transClockPulseAck = “18w : 5 word”;
+Overload transHoldDevAck = “19w : 5 word”;
+Overload popFmtFifo = “20w : 5 word”;
+
 (* Direct translation from @{file "i2cCoreCiruitLib.sml"} *)
 Definition fmt_fifo_reset_def:
-  fmt_fifo_reset (fext : i2c_circuit_ext_state) (s: i2c_circuit_state) (s': i2c_circuit_state) = ^fmt_fifo_reset_tm
+  fmt_fifo_reset (fext : i2c_circuit_ext_state) (s: i2c_circuit_state) (s': i2c_circuit_state) = 
+  s' with fmt_fifo := s'.fmt_fifo with reset := ((s'.reg2hw.fifo_ctrl.fmtrst_q = 1w) ∧ s.reg2hw.fifo_ctrl.fmtrst_qe)
 End
 
 Definition fmt_fifo_rdata_def:
-  fmt_fifo_rdata (fext : i2c_circuit_ext_state) (s: i2c_circuit_state) (s': i2c_circuit_state) = ^fmt_fifo_rdata_tm
+  fmt_fifo_rdata (fext : i2c_circuit_ext_state) (s: i2c_circuit_state) (s': i2c_circuit_state) =
+  s' with fmt_fifo := s'.fmt_fifo with rdata := s.fmt_fifo_regfile $ (5 >< 0) s.fmt_fifo.rptr
 End
 
 Definition fmt_fifo_rready_def:
-  fmt_fifo_rready (fext : i2c_circuit_ext_state) (s: i2c_circuit_state) (s': i2c_circuit_state) = ^fmt_fifo_rready_tm
+  fmt_fifo_rready (fext : i2c_circuit_ext_state) (s: i2c_circuit_state) (s': i2c_circuit_state) =
+  s' with fmt_fifo := s'.fmt_fifo with rready := (s.fsm_state = popFmtFifo)
 End
 
 Definition fmt_fifo_empty_def:
-  fmt_fifo_empty (fext : i2c_circuit_ext_state) (s: i2c_circuit_state) (s': i2c_circuit_state) = ^fmt_fifo_empty_tm
+  fmt_fifo_empty (fext : i2c_circuit_ext_state) (s: i2c_circuit_state) (s': i2c_circuit_state) =
+  s' with fmt_fifo := s'.fmt_fifo with empty := (s.fmt_fifo.rptr = s.fmt_fifo.wptr)
 End
 
 Definition fmt_fifo_incr_rptr_def:
-  fmt_fifo_incr_rptr (fext : i2c_circuit_ext_state) (s: i2c_circuit_state) (s': i2c_circuit_state) = ^fmt_fifo_incr_rptr_tm
+  fmt_fifo_incr_rptr (fext : i2c_circuit_ext_state) (s: i2c_circuit_state) (s': i2c_circuit_state) =
+  s' with fmt_fifo := s'.fmt_fifo with incr_rptr := (¬s'.fmt_fifo.empty ∧ s'.fmt_fifo.rready)
 End
 
 Definition fmt_fifo_counter_rptr_wrap_def:
-  fmt_fifo_counter_rptr_wrap (fext : i2c_circuit_ext_state) (s: i2c_circuit_state) (s': i2c_circuit_state) = ^fmt_fifo_counter_rptr_wrap_tm
+  fmt_fifo_counter_rptr_wrap (fext : i2c_circuit_ext_state) (s: i2c_circuit_state) (s': i2c_circuit_state) =
+  s' with fmt_fifo := s'.fmt_fifo with counter2 := s'.fmt_fifo.counter2 with rptr_wrap :=
+  (s'.fmt_fifo.incr_rptr ∧ (5 >< 0) s.fmt_fifo.rptr = 63w : 6 word)
 End
 
 Definition fmt_fifo_counter_rptr_wrap_cnt_def:
-  fmt_fifo_counter_rptr_wrap_cnt (fext : i2c_circuit_ext_state) (s: i2c_circuit_state) (s': i2c_circuit_state) = ^fmt_fifo_counter_rptr_wrap_cnt_tm
+  fmt_fifo_counter_rptr_wrap_cnt (fext : i2c_circuit_ext_state) (s: i2c_circuit_state) (s': i2c_circuit_state) =
+  s' with fmt_fifo := s'.fmt_fifo with counter2 := s'.fmt_fifo.counter2 with rptr_wrap_cnt :=
+  if ¬ word_bit 6 s.fmt_fifo.rptr then (64w : 7 word) else 0w
 End
 
 Definition fmt_fifo_rptr_ff_def:
-  fmt_fifo_rptr_ff (fext : i2c_circuit_ext_state) (s: i2c_circuit_state) (s': i2c_circuit_state) = ^fmt_fifo_rptr_tm
+  fmt_fifo_rptr_ff (fext : i2c_circuit_ext_state) (s: i2c_circuit_state) (s': i2c_circuit_state) =
+  if s'.fmt_fifo.reset then
+    s' with fmt_fifo := s'.fmt_fifo with rptr := 0w
+  else if s'.fmt_fifo.counter2.rptr_wrap then
+    s' with fmt_fifo := s'.fmt_fifo with rptr := s'.fmt_fifo.counter2.rptr_wrap_cnt
+  else
+    s' with fmt_fifo := s'.fmt_fifo with rptr := s.fmt_fifo.rptr + 1w
 End
 
 Definition fmt_fifo_wvalid_def:
-  fmt_fifo_wvalid (fext : i2c_circuit_ext_state) (s: i2c_circuit_state) (s': i2c_circuit_state) = ^fmt_fifo_wvalid_tm
+  fmt_fifo_wvalid (fext : i2c_circuit_ext_state) (s: i2c_circuit_state) (s': i2c_circuit_state) =
+   s' with fmt_fifo := s'.fmt_fifo with wvalid :=
+   (s.reg2hw.fdata.fbyte_qe ∧ s.reg2hw.fdata.start_qe ∧ s.reg2hw.fdata.stop_qe ∧ s.reg2hw.fdata.read_qe ∧ s.reg2hw.fdata.rcont_qe ∧ s.reg2hw.fdata.nakok_qe)
 End
 
 Definition fmt_fifo_full_def:
-  fmt_fifo_full (fext : i2c_circuit_ext_state) (s: i2c_circuit_state) (s': i2c_circuit_state) = ^fmt_fifo_full_tm
+  fmt_fifo_full (fext : i2c_circuit_ext_state) (s: i2c_circuit_state) (s': i2c_circuit_state) =
+  s' with fmt_fifo := s'.fmt_fifo with full :=
+  ( word_bit 6 s.fmt_fifo.wptr ≠ word_bit 6 s.fmt_fifo.rptr
+    ∧ (5 >< 0) s.fmt_fifo.wptr : 6 word = (5 >< 0) s.fmt_fifo.rptr : 6 word)
 End
 
 Definition fmt_fifo_incr_wptr_def:
-  fmt_fifo_incr_wptr (fext : i2c_circuit_ext_state) (s: i2c_circuit_state) (s': i2c_circuit_state) = ^fmt_fifo_incr_wptr_tm
+  fmt_fifo_incr_wptr (fext : i2c_circuit_ext_state) (s: i2c_circuit_state) (s': i2c_circuit_state) =
+  s' with fmt_fifo := s'.fmt_fifo with incr_wptr := (¬s'.fmt_fifo.full ∧ s'.fmt_fifo.wvalid)
 End
 
 Definition fmt_fifo_wdata_def:
-  fmt_fifo_wdata (fext : i2c_circuit_ext_state) (s: i2c_circuit_state) (s': i2c_circuit_state) = ^fmt_fifo_wdata_tm
+  fmt_fifo_wdata (fext : i2c_circuit_ext_state) (s: i2c_circuit_state) (s': i2c_circuit_state) =
+  s' with fmt_fifo := s'.fmt_fifo with wdata :=
+  (w2w s'.reg2hw.fdata.nakok_q <<~ 12w)
+  || (w2w s'.reg2hw.fdata.rcont_q <<~ 11w)
+  || (w2w s'.reg2hw.fdata.read_q <<~ 10w)
+  || (w2w s'.reg2hw.fdata.stop_q <<~ 9w)
+  || (w2w s'.reg2hw.fdata.start_q <<~ 8w)
+  ||  w2w s'.reg2hw.fdata.fbyte_q
 End
 
 Definition fmt_fifo_regfile_ff_def:
-  fmt_fifo_regfile_ff (fext : i2c_circuit_ext_state) (s: i2c_circuit_state) (s': i2c_circuit_state) = ^fmt_fifo_regfile_tm
+  fmt_fifo_regfile_ff (fext : i2c_circuit_ext_state) (s: i2c_circuit_state) (s': i2c_circuit_state) =
+  let
+    wptr = (5 >< 0) s.fmt_fifo.wptr;
+  in
+    if s'.fmt_fifo.incr_wptr
+    then s' with fmt_fifo_regfile := (wptr =+ s'.fmt_fifo.wdata) s'.fmt_fifo_regfile
+    else s'
 End
 
 Definition fmt_fifo_counter_wptr_wrap_def:
-  fmt_fifo_counter_wptr_wrap (fext : i2c_circuit_ext_state) (s: i2c_circuit_state) (s': i2c_circuit_state) = ^fmt_fifo_counter_wptr_wrap_tm
+  fmt_fifo_counter_wptr_wrap (fext : i2c_circuit_ext_state) (s: i2c_circuit_state) (s': i2c_circuit_state) =
+  s' with fmt_fifo := s'.fmt_fifo with counter2 := s'.fmt_fifo.counter2 with wptr_wrap :=
+  (s'.fmt_fifo.incr_wptr ∧ (5 >< 0) s.fmt_fifo.wptr = 63w : 6 word)
 End
 
 Definition fmt_fifo_counter_wptr_wrap_cnt_def:
-  fmt_fifo_counter_wptr_wrap_cnt (fext : i2c_circuit_ext_state) (s: i2c_circuit_state) (s': i2c_circuit_state) = ^fmt_fifo_counter_wptr_wrap_cnt_tm
+  fmt_fifo_counter_wptr_wrap_cnt (fext : i2c_circuit_ext_state) (s: i2c_circuit_state) (s': i2c_circuit_state) =
+  s' with fmt_fifo := s'.fmt_fifo with counter2 := s'.fmt_fifo.counter2 with wptr_wrap_cnt :=
+  if ¬ (word_bit 6 s.fmt_fifo.wptr) then 64w else 0w
 End
 
 Definition fmt_fifo_wptr_ff_def:
-  fmt_fifo_wptr_ff (fext : i2c_circuit_ext_state) (s: i2c_circuit_state) (s': i2c_circuit_state) = ^fmt_fifo_wptr_tm
+  fmt_fifo_wptr_ff (fext : i2c_circuit_ext_state) (s: i2c_circuit_state) (s': i2c_circuit_state) =
+  if s'.fmt_fifo.reset then
+    s' with fmt_fifo := s'.fmt_fifo with wptr := 0w
+  else if s'.fmt_fifo.counter2.wptr_wrap then
+    s' with fmt_fifo := s'.fmt_fifo with wptr := s'.fmt_fifo.counter2.wptr_wrap_cnt
+  else
+    s' with fmt_fifo := s'.fmt_fifo with wptr := s.fmt_fifo.wptr + 1w
 End
 
 Definition i2c_core_delay_comb_def:
   i2c_core_delay_comb (fext: i2c_circuit_ext_state) (s: i2c_circuit_state) (s': i2c_circuit_state) =
-  ^delay_tm
+  let
+    s' = s' with delay := s'.delay with setup_start := w2w s.regs.timing1.t_r + w2w s.regs.timing2.tsu_sta ;
+    s' = s' with delay := s'.delay with hold_start  := w2w s.regs.timing1.t_f + w2w s.regs.timing2.thd_sta ;
+    s' = s' with delay := s'.delay with setup_data  := w2w s.regs.timing1.t_r + w2w s.regs.timing3.tsu_dat ;
+    s' = s' with delay := s'.delay with clock_start := w2w s.regs.timing3.thd_dat ;
+    s' = s' with delay := s'.delay with clock_low   := w2w s.regs.timing0.tlow - w2w s.regs.timing3.thd_dat;
+    s' = s' with delay := s'.delay with clock_pulse := w2w s.regs.timing1.t_r + w2w s.regs.timing0.thigh + w2w s.regs.timing1.t_f ;
+    s' = s' with delay := s'.delay with hold_bit    := w2w s.regs.timing1.t_f + w2w s.regs.timing3.thd_dat ;
+    s' = s' with delay := s'.delay with clock_stop  := w2w s.regs.timing1.t_f + w2w s.regs.timing0.tlow - w2w s.regs.timing3.thd_dat ;
+    s' = s' with delay := s'.delay with setup_stop  := w2w s.regs.timing1.t_r + w2w s.regs.timing4.tsu_sto ;
+    s' = s' with delay := s'.delay with hold_stop   := w2w s.regs.timing1.t_r + w2w s.regs.timing4.t_buf - w2w s.regs.timing2.tsu_sta ;
+  in
+    s'
 End
 
 Definition i2c_core_curr_delay_comb_def:
   i2c_core_curr_delay_comb (fext: i2c_circuit_ext_state) (s: i2c_circuit_state) (s': i2c_circuit_state) =
-  ^curr_delay_tm
+  case s.fsm_state of
+    recReadClockLow      => s' with curr_delay := s'.delay.clock_low
+  | recReadClockPulse    => s' with curr_delay := s'.delay.clock_pulse
+  | recReadHoldBit       => s' with curr_delay := s'.delay.hold_bit
+  | recHostClockLowAck   => s' with curr_delay := s'.delay.clock_low
+  | recHostClockPulseAck => s' with curr_delay := s'.delay.clock_pulse
+  | recHostHoldBitAck    => s' with curr_delay := s'.delay.hold_bit
+  | stopClockStop        => s' with curr_delay := s'.delay.clock_stop
+  | stopSetupStop        => s' with curr_delay := s'.delay.setup_stop
+  | stopHoldStop         => s' with curr_delay := s'.delay.hold_stop
+  | startSetupStart      => s' with curr_delay := s'.delay.setup_start
+  | startHoldStart       => s' with curr_delay := s'.delay.hold_start
+  | startClockStart      => s' with curr_delay := s'.delay.clock_start
+  | transClockLow        => s' with curr_delay := s'.delay.clock_low
+  | transClockPulse      => s' with curr_delay := s'.delay.clock_pulse
+  | transHoldBit         => s' with curr_delay := s'.delay.hold_bit
+  | transClockLowAck     => s' with curr_delay := s'.delay.clock_low
+  | transClockPulseAck   => s' with curr_delay := s'.delay.clock_pulse
+  | transHoldDevAck      => s' with curr_delay := s'.delay.hold_bit
+  | _                    => s' with curr_delay := 0w
 End
 
 Definition i2c_core_load_tcount_comb_def:
   i2c_core_load_tcount_comb (fext: i2c_circuit_ext_state) (s: i2c_circuit_state) (s': i2c_circuit_state) =
-  ^load_tcount_tm
+  s' with load_tcount := (s.fsm_state ≠ idle ∧ s.counter = 1w ∨ s.fsm_state = popFmtFifo)
 End
 
 Definition i2c_core_log_start_comb_def:
   i2c_core_log_start_comb (fext : i2c_circuit_ext_state) (s : i2c_circuit_state) (s' : i2c_circuit_state) =
-  ^log_start_tm
+  s' with log_start := (s.fsm_state = startSetupStart ∧ s.counter = 1w)
 End
 
 Definition i2c_core_log_stop_comb_def:
   i2c_core_log_stop_comb (fext : i2c_circuit_ext_state) (s : i2c_circuit_state) (s' : i2c_circuit_state) =
-  ^log_stop_tm
+  s' with log_stop := (s.fsm_state = stopClockStop ∧ s.counter = 1w)
 End
 
 Definition fmt_fifo_rvalid_def:
-  fmt_fifo_rvalid (fext : i2c_circuit_ext_state) (s: i2c_circuit_state) (s': i2c_circuit_state) = ^fmt_fifo_rvalid_tm
+  fmt_fifo_rvalid (fext : i2c_circuit_ext_state) (s: i2c_circuit_state) (s': i2c_circuit_state) =
+  s' with fmt_fifo := s'.fmt_fifo with rvalid := ¬s'.fmt_fifo.empty
 End
 
 Definition fmt_fifo_flag_start_before_def:
-  fmt_fifo_flag_start_before (fext : i2c_circuit_ext_state) (s: i2c_circuit_state) (s': i2c_circuit_state) = ^fmt_fifo_flag_start_before_tm
+  fmt_fifo_flag_start_before (fext : i2c_circuit_ext_state) (s: i2c_circuit_state) (s': i2c_circuit_state) =
+  s' with fmt_flag := s'.fmt_flag with start_before :=
+  (s'.fmt_fifo.rvalid ∧ word_bit 8 s'.fmt_fifo.rdata)
 End
 
 Definition fmt_fifo_flag_stop_after_def:
-  fmt_fifo_flag_stop_after (fext : i2c_circuit_ext_state) (s: i2c_circuit_state) (s': i2c_circuit_state) = ^fmt_fifo_flag_stop_after_tm
+  fmt_fifo_flag_stop_after (fext : i2c_circuit_ext_state) (s: i2c_circuit_state) (s': i2c_circuit_state) =
+  s' with fmt_flag := s'.fmt_flag with stop_after :=
+  (s'.fmt_fifo.rvalid ∧ word_bit 9 s'.fmt_fifo.rdata)
 End
 
 Definition fmt_fifo_flag_read_bytes_def:
-  fmt_fifo_flag_read_bytes (fext : i2c_circuit_ext_state) (s: i2c_circuit_state) (s': i2c_circuit_state) = ^fmt_fifo_flag_read_bytes_tm
+  fmt_fifo_flag_read_bytes (fext : i2c_circuit_ext_state) (s: i2c_circuit_state) (s': i2c_circuit_state) =
+  s' with fmt_flag := s'.fmt_flag with read_bytes :=
+  (s'.fmt_fifo.rvalid ∧ word_bit 10 s'.fmt_fifo.rdata)
+End
+
+Definition fmt_fifo_flag_nak_ok_def:
+  fmt_fifo_flag_nak_ok (fext : i2c_circuit_ext_state) (s: i2c_circuit_state) (s': i2c_circuit_state) =
+  s' with fmt_flag := s'.fmt_flag with nak_ok :=
+  (s'.fmt_fifo.rvalid ∧ word_bit 12 s'.fmt_fifo.rdata)
 End
 
 Definition fmt_byte_def:
-  fmt_byte (fext : i2c_circuit_ext_state) (s: i2c_circuit_state) (s': i2c_circuit_state) = ^fmt_byte_tm
+  fmt_byte (fext : i2c_circuit_ext_state) (s: i2c_circuit_state) (s': i2c_circuit_state) =
+  s' with fmt_byte :=
+  if s'.fmt_fifo.rvalid then (7 >< 0) s'.fmt_fifo.rdata else 0w
 End
 
 Definition req_restart_def:
-  req_restart (fext : i2c_circuit_ext_state) (s: i2c_circuit_state) (s': i2c_circuit_state) = ^req_restart_tm
+  req_restart (fext : i2c_circuit_ext_state) (s: i2c_circuit_state) (s': i2c_circuit_state) =
+  s' with req_restart := ( ¬s'.fmt_flag.read_bytes ∧  s'.fmt_flag.start_before
+                           ∧  s.fsm_state = active ∧  s.trans_started )
 End
 
 Definition bit_clr_def:
-  bit_clr (fext: i2c_circuit_ext_state) (s: i2c_circuit_state) (s': i2c_circuit_state) = ^bit_clr_tm
+  bit_clr (fext: i2c_circuit_ext_state) (s: i2c_circuit_state) (s': i2c_circuit_state) =
+  s' with bit_clr := ( (s.fsm_state = transHoldBit ∨ s.fsm_state = recReadHoldBit)
+                       ∧  s.counter = 1w ∧ s.bit_index = 0w )
 End
 
 Definition bit_decr_def:
-  bit_decr (fext: i2c_circuit_ext_state) (s: i2c_circuit_state) (s': i2c_circuit_state) = ^bit_decr_tm
+  bit_decr (fext: i2c_circuit_ext_state) (s: i2c_circuit_state) (s': i2c_circuit_state) =
+  s' with bit_decr := ((s.fsm_state = transHoldBit ∨ s.fsm_state = recReadHoldBit)
+                       ∧ s.counter = 1w ∧ s.bit_index ≠ 0w )
 End
 
 Definition i2c_core_stretch_en_comb_def:
   i2c_core_stretch_en_comb (fext: i2c_circuit_ext_state) (s: i2c_circuit_state) (s': i2c_circuit_state) =
-  ^stretch_en_tm
-End
-
-Definition stretch_en_def:
-  stretch_en (fext: i2c_circuit_ext_state) (s: i2c_circuit_state) (s': i2c_circuit_state) = ^stretch_en_tm
+  s' with stretch_en := (s.fsm_state = transClockPulse ∨  s.fsm_state = transClockPulseAck
+                         ∨  s.fsm_state = recReadClockPulse ∨  s.fsm_state = recHostClockPulseAck)
 End
 
 Definition i2c_core_scl_d_comb_def:
-  i2c_core_scl_d_comb (fext: i2c_circuit_ext_state) (s: i2c_circuit_state) (s': i2c_circuit_state) = ^scl_d_tm
+  i2c_core_scl_d_comb (fext: i2c_circuit_ext_state) (s: i2c_circuit_state) (s': i2c_circuit_state) =
+  s' with scl_d := ¬( s.fsm_state = startClockStart
+                      ∨ s.fsm_state = transClockLow
+                      ∨ s.fsm_state = transHoldBit
+                      ∨ s.fsm_state = transClockLowAck
+                      ∨ s.fsm_state = transHoldDevAck
+                      ∨ s.fsm_state = recReadClockLow
+                      ∨ s.fsm_state = recReadHoldBit
+                      ∨ s.fsm_state = recHostClockLowAck
+                      ∨ s.fsm_state = recHostHoldBitAck
+                      ∨ s.fsm_state = recHostHoldBitAck
+                      ∨ s.fsm_state = stopClockStop
+                      ∨ s.fsm_state = active ∧ (¬s'.fmt_flag.start_before ∨ s.trans_started)
+                      ∨ s.fsm_state = popFmtFifo ∧ ¬s'.fmt_flag.stop_after)
 End
 
 Definition i2c_core_next_scl_rx_val_comb_def:
-  i2c_core_next_scl_rx_val_comb (fext : i2c_circuit_ext_state) (s: i2c_circuit_state) (s': i2c_circuit_state) = ^next_scl_rx_val_tm
+  i2c_core_next_scl_rx_val_comb (fext : i2c_circuit_ext_state) (s: i2c_circuit_state) (s': i2c_circuit_state) =
+  if fext.cio_scl_i then
+    s' with next_scl_rx_val := (w2w s.scl_rx_val <<~ 1w) || 1w
+  else
+    s' with next_scl_rx_val := (w2w s.scl_rx_val <<~ 1w)
 End
 
 Definition i2c_core_next_stretch_idle_cnt_def:
   i2c_core_next_stretch_idle_cnt (fext: i2c_circuit_ext_state) (s: i2c_circuit_state) (s': i2c_circuit_state) =
-  ^next_stretch_idle_cnt_tm
+  if s'.stretch_en ∧ s'.scl_d ∧ ¬fext.cio_scl_i
+  then s' with next_stretch_idle_cnt := s.stretch_idle_cnt + 1w
+  else s' with next_stretch_idle_cnt := 0w
 End
 
 Definition i2c_core_next_counter_def:
   i2c_core_next_counter (fext: i2c_circuit_ext_state) (s: i2c_circuit_state) (s': i2c_circuit_state) =
-  ^next_counter_tm
+  if s'.load_tcount then s' with next_counter := s'.curr_delay
+  else if s.stretch_idle_cnt = 0w then s' with next_counter := s.counter - 1w
+  else s' with next_counter := s.counter
 End
 
 Definition i2c_core_byte_clr_comb_def:
   i2c_core_byte_clr_comb (fext: i2c_circuit_ext_state) (s: i2c_circuit_state) (s': i2c_circuit_state) =
-  ^byte_clr_tm
+  s' with byte_clr := (s.fsm_state = active ∧ s'.fmt_flag.read_bytes)
 End
 
 Definition i2c_core_byte_decr_comb_def:
   i2c_core_byte_decr_comb (fext: i2c_circuit_ext_state) (s: i2c_circuit_state) (s': i2c_circuit_state) =
-  ^byte_decr_tm
+  s' with byte_decr := (s.fsm_state = recHostHoldBitAck ∧ s.counter = 1w ∧ s.byte_index ≠ 1w)
 End
 
 Definition i2c_core_byte_num_comb_def:
   i2c_core_byte_num_comb (fext: i2c_circuit_ext_state) (s: i2c_circuit_state) (s': i2c_circuit_state) =
-  ^byte_num_tm
+  if ¬s'.fmt_flag.read_bytes then s' with byte_num := 0w
+  else if s'.fmt_byte = 0w then s' with byte_num := 256w
+  else s' with byte_num := w2w s'.fmt_byte
 End
 
 Definition i2c_core_next_byte_index_comb_def:
   i2c_core_next_byte_index_comb (fext: i2c_circuit_ext_state) (s: i2c_circuit_state) (s': i2c_circuit_state) =
-  ^next_byte_index_tm
+  if s'.byte_clr then s' with next_byte_index := s'.byte_num
+  else if s'.byte_decr then s' with next_byte_index := s.byte_index - 1w
+  else s' with next_byte_index := s.byte_index
 End
 
 Definition fifo_depth_def:
   fifo_depth (fext: i2c_circuit_ext_state) (s: i2c_circuit_state) (s':i2c_circuit_state) =
-  ^fifo_depth_tm
+  if s'.fmt_fifo.full then
+    s' with fmt_fifo := s'.fmt_fifo with depth := 64w
+  else if word_bit 6 s.fmt_fifo.wptr = word_bit 6 s.fmt_fifo.rptr then
+    s' with fmt_fifo := s'.fmt_fifo with depth :=
+    ((w2w ((5 >< 0) s.fmt_fifo.wptr : 6 word)) - (w2w ((5 >< 0) s.fmt_fifo.rptr : 6 word)))
+  else
+    s' with fmt_fifo := s'.fmt_fifo with depth :=
+    64w - w2w ((5 >< 0) s.fmt_fifo.rptr : 6 word) + w2w ((5 >< 0) s.fmt_fifo.wptr :  6 word)
 End
 
 Definition counter_gt_one_comb_def:
   counter_gt_one_comb (fext: i2c_circuit_ext_state) (s: i2c_circuit_state) (s':i2c_circuit_state) =
-  ^counter_gt_one_tm
+  s' with cnt_gt_one := (1w <+ s.counter)
 End
 
 Definition i2c_core_next_state_def:
   i2c_core_next_state (fext: i2c_circuit_ext_state) (s: i2c_circuit_state) (s': i2c_circuit_state) =
-  ^next_state_tm
+  case s.fsm_state of
+    idle                 => if s.regs.ctrl.enablehost = 1w ∧ s'.fmt_fifo.rvalid
+                            then s' with next_state := active
+                            else s' with next_state := idle
+  | active               => if s'.fmt_flag.read_bytes then
+                              s' with next_state := recReadClockLow
+                            else if s'.fmt_flag.start_before ∧ ¬s.trans_started then
+                              s' with next_state := startSetupStart
+                            else
+                              s' with next_state := transClockLow
+
+  | recReadClockLow      => if s'.cnt_gt_one then s' with next_state := recReadClockLow
+                            else s' with next_state := recReadClockPulse
+
+  | recReadClockPulse    => if s'.cnt_gt_one then s' with next_state := recReadClockPulse
+                            else s' with next_state := recReadHoldBit
+
+  | recReadHoldBit       => if s'.cnt_gt_one then
+                              s' with next_state := recReadHoldBit
+                            else if s.bit_index = 0w then
+                              s' with next_state := recHostClockLowAck
+                            else
+                              s' with next_state := recReadClockLow
+
+  | recHostClockLowAck   => if s'.cnt_gt_one then s' with next_state := recHostClockLowAck
+                            else s' with next_state := recHostClockPulseAck
+
+  | recHostClockPulseAck => if s'.cnt_gt_one then s' with next_state := recHostClockPulseAck
+                            else s' with next_state := recHostHoldBitAck
+
+  | recHostHoldBitAck    => if s'.cnt_gt_one then
+                              s' with next_state := recHostHoldBitAck
+                            else if s.byte_index = 1w ∧ s'.fmt_flag.stop_after then
+                              s' with next_state := stopClockStop
+                            else if s.byte_index = 1w ∧ ¬s'.fmt_flag.stop_after then
+                              s' with next_state := popFmtFifo
+                            else
+                              s' with next_state := recReadClockLow
+
+  | stopClockStop        => if s'.cnt_gt_one then s' with next_state := stopClockStop
+                            else s' with next_state := stopSetupStop
+
+  | stopSetupStop        => if s'.cnt_gt_one then s' with next_state := stopSetupStop
+                            else s' with next_state := stopHoldStop
+
+  | stopHoldStop         => if s'.cnt_gt_one then s' with next_state := stopHoldStop
+                            else if s.regs.ctrl.enablehost = 0w then s' with next_state := idle
+                            else s' with next_state := popFmtFifo
+
+  | startSetupStart      => if s'.cnt_gt_one then s' with next_state := startSetupStart
+                            else s' with next_state := startHoldStart
+
+  | startHoldStart       => if s'.cnt_gt_one then s' with next_state := startHoldStart
+                            else s' with next_state := startClockStart
+
+  | startClockStart      => if s'.cnt_gt_one then s' with next_state := startClockStart
+                            else s' with next_state := transClockLow
+
+  | transClockLow        => if s'.cnt_gt_one then s' with next_state := transClockLow
+                            else if s.pend_restart then s' with next_state := startSetupStart
+                            else s' with next_state := transClockPulse
+
+  | transClockPulse      => if s'.cnt_gt_one then s' with next_state := transClockPulse
+                            else s' with next_state := transHoldBit
+
+  | transHoldBit         => if s'.cnt_gt_one then s' with next_state := transHoldBit
+                            else if s.bit_index = 0w then s' with next_state := transClockLowAck
+                            else s' with next_state := transClockLow
+
+  | transClockLowAck     => if s'.cnt_gt_one then s' with next_state := transClockLowAck
+                            else s' with next_state := transClockPulseAck
+                                                       
+  | transClockPulseAck   => if s'.cnt_gt_one then s' with next_state := transClockPulseAck
+                            else s' with next_state := transHoldDevAck
+
+  | transHoldDevAck      => if s'.cnt_gt_one then
+                              s' with next_state := transHoldDevAck
+                            else if s'.fmt_flag.stop_after then
+                              s' with next_state := stopClockStop
+                            else
+                              s' with next_state := popFmtFifo
+
+  | popFmtFifo           => if s.regs.ctrl.enablehost = 0w then s' with next_state := stopClockStop
+                            else if s'.fmt_fifo.depth = 1w then s' with next_state := idle
+                            else s' with next_state := active
+
+  | _ => s' with next_state := idle
 End
 
 Definition i2c_core_read_byte_clr_comb_def:
   i2c_core_read_byte_clr_comb (fext: i2c_circuit_ext_state) (s: i2c_circuit_state) (s': i2c_circuit_state) =
-  ^read_byte_clr_tm
+  s' with read_byte_clr := (s.fsm_state = recReadHoldBit ∧ s.counter = 1w ∧ s.bit_index = 0w)
 End
 
 Definition i2c_core_shift_data_en_comb_def:
   i2c_core_shift_data_en_comb (fext: i2c_circuit_ext_state) (s: i2c_circuit_state) (s': i2c_circuit_state) =
-  ^shift_data_en_tm
+  s' with shift_data_en := (s.fsm_state = recReadClockPulse ∧ s.counter = 1w)
 End
 
 Definition i2c_core_next_sda_rx_val_comb_def:
   i2c_core_next_sda_rx_val_comb (fext: i2c_circuit_ext_state) (s: i2c_circuit_state) (s': i2c_circuit_state) =
-  ^next_sda_rx_val_tm
+  if fext.cio_sda_i then
+    s' with next_sda_rx_val := (w2w s.sda_rx_val <<~ 1w) || 1w
+  else
+    s' with next_sda_rx_val := (w2w s.sda_rx_val <<~ 1w)
 End
 
 Definition i2c_core_next_read_byte_comb_def:
   i2c_core_next_read_byte_comb (fext: i2c_circuit_ext_state) (s: i2c_circuit_state) (s': i2c_circuit_state) =
-  ^next_read_byte_tm
+  if s'.read_byte_clr then s' with next_read_byte := 0w
+  else if s'.shift_data_en ∧ fext.cio_sda_i then
+    s' with next_read_byte := (w2w s.read_byte <<~ 1w) || 1w
+  else if s'.shift_data_en ∧ ¬fext.cio_sda_i then
+    s' with next_read_byte := (w2w s.read_byte <<~ 1w)
+  else
+    s' with next_read_byte := s.read_byte
 End
 
 Definition i2c_core_rx_fifo_reset_comb_def:
   i2c_core_rx_fifo_reset_comb (fext: i2c_circuit_ext_state) (s: i2c_circuit_state) (s': i2c_circuit_state) =
-  ^rx_fifo_reset_tm
+  s' with rx_fifo := s'.rx_fifo with reset :=
+  (word_bit 0 s'.reg2hw.fifo_ctrl.rxrst_q ∧ s.reg2hw.fifo_ctrl.rxrst_qe)
 End
 
 Definition i2c_core_rx_fifo_rdata_comb_def:
   i2c_core_rx_fifo_rdata_comb (fext: i2c_circuit_ext_state) (s: i2c_circuit_state) (s': i2c_circuit_state) =
-  ^rx_fifo_rdata_tm
+  s' with rx_fifo := s'.rx_fifo with rdata := s.rx_fifo_regfile $ (5 >< 0) s.rx_fifo.rptr
 End
 
 Definition i2c_core_rx_fifo_rready_comb_def:
   i2c_core_rx_fifo_rready_comb (fext: i2c_circuit_ext_state) (s: i2c_circuit_state) (s': i2c_circuit_state) =
-  ^rx_fifo_rready_tm
+  s' with rx_fifo := s'.rx_fifo with rready := s'.reg2hw.rdata.rdata_re
 End
 
 Definition i2c_core_rx_fifo_empty_comb_def:
   i2c_core_rx_fifo_empty_comb (fext: i2c_circuit_ext_state) (s: i2c_circuit_state) (s': i2c_circuit_state) =
-  ^rx_fifo_empty_tm
+  s' with rx_fifo := s'.rx_fifo with empty := (s.rx_fifo.rptr = s.rx_fifo.wptr)
 End
 
 Definition i2c_core_rx_fifo_incr_rptr_comb_def:
   i2c_core_rx_fifo_incr_rptr_comb (fext: i2c_circuit_ext_state) (s: i2c_circuit_state) (s': i2c_circuit_state) =
-  ^rx_fifo_incr_rptr_tm
+  s' with rx_fifo := s'.rx_fifo with incr_rptr := (¬s'.rx_fifo.empty ∧ s'.rx_fifo.rready)
 End
 
 Definition i2c_core_rx_fifo_counter_rptr_wrap_comb_def:
   i2c_core_rx_fifo_counter_rptr_wrap_comb (fext: i2c_circuit_ext_state) (s: i2c_circuit_state) (s': i2c_circuit_state) =
-  ^rx_fifo_counter_rptr_wrap_tm
+  s' with rx_fifo := s'.rx_fifo with counter := s'.rx_fifo.counter with rptr_wrap :=
+  (s'.rx_fifo.incr_rptr ∧ (5 >< 0) s.rx_fifo.rptr = 63w : 6 word)
 End
 
 Definition i2c_core_rx_fifo_counter_rptr_wrap_cnt_comb_def:
   i2c_core_rx_fifo_counter_rptr_wrap_cnt_comb (fext: i2c_circuit_ext_state) (s: i2c_circuit_state) (s': i2c_circuit_state) =
-  ^rx_fifo_counter_rptr_wrap_cnt_tm
+  s' with rx_fifo := s'.rx_fifo with counter := s'.rx_fifo.counter with rptr_wrap_cnt :=
+  if ¬ word_bit 6 s.rx_fifo.rptr then (64w : 7 word) else 0w
 End
 
 Definition i2c_core_rx_fifo_rptr_ff_def:
   i2c_core_rx_fifo_rptr_ff (fext: i2c_circuit_ext_state) (s: i2c_circuit_state) (s': i2c_circuit_state) =
-  ^rx_fifo_counter_rptr_wrap_cnt_tm
+  if s'.rx_fifo.reset then
+    s' with rx_fifo := s'.rx_fifo with rptr := 0w
+  else if s'.rx_fifo.counter.rptr_wrap then
+    s' with rx_fifo := s'.rx_fifo with rptr := s'.rx_fifo.counter.rptr_wrap_cnt
+  else
+    s' with rx_fifo := s'.rx_fifo with rptr := s.rx_fifo.rptr + 1w
 End
 
 Definition i2c_core_rx_fifo_wvalid_comb_def:
   i2c_core_rx_fifo_wvalid_comb (fext: i2c_circuit_ext_state) (s: i2c_circuit_state) (s': i2c_circuit_state) =
-  ^rx_fifo_wvalid_tm
+  s' with rx_fifo := s'.rx_fifo with wvalid :=
+  (s.fsm_state = recReadHoldBit ∧ s.bit_index = 0w ∧ s.counter = 1w)
 End
 
 Definition i2c_core_rx_fifo_wdata_comb_def:
   i2c_core_rx_fifo_wdata_comb (fext: i2c_circuit_ext_state) (s: i2c_circuit_state) (s': i2c_circuit_state) =
-  ^rx_fifo_wdata_tm
+  if s.fsm_state = recReadHoldBit ∧ s.bit_index = 0w ∧ s.counter = 1w then
+    s' with rx_fifo := s'.rx_fifo with wdata := s.read_byte
+  else
+    s' with rx_fifo := s'.rx_fifo with wdata := 0w
 End
 
 Definition i2c_core_rx_fifo_full_comb_def:
   i2c_core_rx_fifo_full_comb (fext: i2c_circuit_ext_state) (s: i2c_circuit_state) (s': i2c_circuit_state) =
-  ^rx_fifo_full_tm
+  s' with rx_fifo := s'.rx_fifo with full :=
+  ((word_bit 5 s.rx_fifo.wptr ≠ word_bit 5 s.rx_fifo.rptr) ∧
+   ((5 >< 0) s.rx_fifo.wptr : 6 word = (5 >< 0) s.rx_fifo.rptr : 6 word))
 End
 
 Definition i2c_core_rx_fifo_incr_wptr_comb_def:
   i2c_core_rx_fifo_incr_wptr_comb (fext: i2c_circuit_ext_state) (s: i2c_circuit_state) (s': i2c_circuit_state) =
-  ^rx_fifo_incr_wptr_tm
+  s' with rx_fifo := s'.rx_fifo with incr_wptr := (¬s'.rx_fifo.full ∧ s'.rx_fifo.wvalid)
 End
 
 Definition i2c_core_rx_fifo_regfile_def:
   i2c_core_rx_fifo_regfile (fext: i2c_circuit_ext_state) (s: i2c_circuit_state) (s': i2c_circuit_state) =
-  ^rx_fifo_regfile_tm
+  let
+    wptr = (5 >< 0) s.rx_fifo.wptr;
+  in
+    if s'.rx_fifo.incr_wptr
+    then s' with rx_fifo_regfile := (wptr =+ s'.rx_fifo.wdata) s'.rx_fifo_regfile
+    else s'
 End
 
 Definition i2c_core_rx_fifo_counter_wptr_wrap_comb_def:
   i2c_core_rx_fifo_counter_wptr_wrap_comb (fext: i2c_circuit_ext_state) (s: i2c_circuit_state) (s': i2c_circuit_state) =
-  ^rx_fifo_counter_wptr_wrap_tm
+  s' with rx_fifo := s'.rx_fifo with counter := s'.rx_fifo.counter with wptr_wrap :=
+  (s'.rx_fifo.incr_wptr ∧ (5 >< 0) s.rx_fifo.wptr = 63w : 6 word)
 End
 
 Definition i2c_core_rx_fifo_counter_wptr_wrap_cnt_comb_def:
   i2c_core_rx_fifo_counter_wptr_wrap_cnt_comb (fext: i2c_circuit_ext_state) (s: i2c_circuit_state) (s': i2c_circuit_state) =
-  ^rx_fifo_counter_wptr_wrap_cnt_tm
+  s' with rx_fifo := s'.rx_fifo with counter := s'.rx_fifo.counter with wptr_wrap_cnt :=
+  if ¬word_bit 6 s.rx_fifo.wptr then 64w else 0w
 End
 
 Definition i2c_core_rx_fifo_wptr_ff_def:
   i2c_core_rx_fifo_wptr_ff (fext: i2c_circuit_ext_state) (s: i2c_circuit_state) (s': i2c_circuit_state) =
-  ^rx_fifo_wptr_tm
+  if s'.rx_fifo.reset then
+    s' with rx_fifo := s'.rx_fifo with wptr := 0w
+  else if s'.rx_fifo.counter.wptr_wrap then
+    s' with rx_fifo := s'.rx_fifo with wptr := s'.rx_fifo.counter.wptr_wrap_cnt
+  else
+    s' with rx_fifo := s'.rx_fifo with wptr := s.rx_fifo.wptr + 1w
 End
 
 Definition hw2reg_intr_state_nak_de_comb_def:
   hw2reg_intr_state_nak_de_comb (fext: i2c_circuit_ext_state) (s: i2c_circuit_state) (s': i2c_circuit_state) =
-  ^hw2reg_intr_state_nak_de_tm
+  s' with hw2reg := s'.hw2reg with intr_state := s'.hw2reg.intr_state with nak_de :=
+  (s.fsm_state = transClockPulseAck ∧ ¬s'.fmt_flag.nak_ok ∧ fext.cio_sda_i)
 End
 
 Definition hw2reg_intr_state_nak_d_comb_def:
   hw2reg_intr_state_nak_d_comb (fext: i2c_circuit_ext_state) (s: i2c_circuit_state) (s': i2c_circuit_state) =
-  ^hw2reg_intr_state_nak_d_tm
+  s' with hw2reg := s'.hw2reg with intr_state := s'.hw2reg.intr_state with nak_d :=
+  n2w $ bool_to_bit
+      ( s.fsm_state = transClockPulseAck ∧ ¬s'.fmt_flag.nak_ok ∧ fext.cio_sda_i
+        ∨ word_bit 0 s'.reg2hw.intr_state.nak_q)
 End
 
 Definition next_intr_nak_comb_def:
   next_intr_nak_comb (fext: i2c_circuit_ext_state) (s: i2c_circuit_state) (s': i2c_circuit_state) =
-  ^next_intr_nak_o_tm
+  s' with next_intr_nak_o := (word_bit 0 s'.reg2hw.intr_state.nak_q ∧ word_bit 0 s'.reg2hw.intr_enable.nak_q)
 End
 
 Definition hw2reg_intr_state_cmd_complete_de_comb_def:
   hw2reg_intr_state_cmd_complete_de_comb (fext: i2c_circuit_ext_state) (s: i2c_circuit_state) (s': i2c_circuit_state) =
-  ^hw2reg_intr_state_cmd_complete_de_tm
+  s' with hw2reg := s'.hw2reg with intr_state := s'.hw2reg.intr_state with cmd_complete_de :=
+  (s.fsm_state = stopHoldStop ∨ s.fsm_state = startSetupStart ∧ s'.log_start ∧ s.pend_restart)
 End
 
 Definition hw2reg_intr_state_cmd_complete_d_comb_def:
   hw2reg_intr_state_cmd_complete_d_comb (fext: i2c_circuit_ext_state) (s: i2c_circuit_state) (s': i2c_circuit_state) =
-  ^hw2reg_intr_state_cmd_complete_d_tm
+  s' with hw2reg := s'.hw2reg with intr_state := s'.hw2reg.intr_state with cmd_complete_d :=
+  if ( s.fsm_state = stopHoldStop ∨ s.fsm_state = startSetupStart ∧ s'.log_start ∧ s.pend_restart
+       ∨ word_bit 0 s'.reg2hw.intr_state.cmd_complete_q ) then 1w else 0w
 End
 
 Definition next_intr_cmd_complete_comb_def:
   next_intr_cmd_complete_comb (fext: i2c_circuit_ext_state) (s: i2c_circuit_state) (s': i2c_circuit_state) =
-  ^next_intr_cmd_complete_o_tm
+  s' with next_intr_cmd_complete_o := (word_bit 0 s'.reg2hw.intr_state.cmd_complete_q ∧ word_bit 0 s'.reg2hw.intr_enable.cmd_complete_q)
 End
 
 Definition next_pend_restart_comb_def:
   next_pend_restart_comb (fext: i2c_circuit_ext_state) (s: i2c_circuit_state) (s':i2c_circuit_state) =
-  ^next_pend_restart_tm
+  if s.pend_restart ∧ s.regs.ctrl.enablehost = 0w ∨ s'.log_start then s' with next_pend_restart := F
+  else if s'.req_restart then s' with next_pend_restart := T
+  else s' with next_pend_restart := s.pend_restart
 End
 
 Definition next_trans_started_comb_def:
   next_trans_started_comb (fext: i2c_circuit_ext_state) (s: i2c_circuit_state) (s':i2c_circuit_state) =
-  ^next_trans_started_tm
+  if s.trans_started ∧ s.regs.ctrl.enablehost = 0w ∨ s'.log_stop then s' with next_trans_started := F
+  else if s'.log_start then s' with next_trans_started := T
+  else s' with next_trans_started := s.trans_started
 End
 
 Definition next_bit_index_comb_def:
   next_bit_index_comb (fext: i2c_circuit_ext_state) (s: i2c_circuit_state) (s':i2c_circuit_state) =
-  ^next_bit_index_tm
+  if s'.bit_clr then s' with next_bit_index := 7w
+  else if s'.bit_decr then s' with next_bit_index := s.bit_index - 1w
+  else s' with next_bit_index := s.bit_index
 End
 
 Definition i2c_core_ff_def:
   i2c_core_ff (fext : i2c_circuit_ext_state) (s: i2c_circuit_state) (s': i2c_circuit_state) =
-  ^i2c_core_ff_tm
+  s' with fsm_state := s'.next_state
 End
 
 Definition i2c_core_counter_ff_def:
   i2c_core_counter_ff (fext: i2c_circuit_ext_state) (s: i2c_circuit_state) (s': i2c_circuit_state) =
-  ^i2c_core_counter_ff_tm
+  s' with counter := s'.next_counter
 End
 
 Definition i2c_core_stretch_idle_cnt_ff_def:
   i2c_core_stretch_idle_cnt_ff (fext: i2c_circuit_ext_state) (s: i2c_circuit_state) (s': i2c_circuit_state) =
-  ^i2c_core_stretch_idle_cnt_ff_tm
+  s' with stretch_idle_cnt := s'.next_stretch_idle_cnt
 End
 
 Definition bit_index_ff_def:
   bit_index_ff (fext: i2c_circuit_ext_state) (s: i2c_circuit_state) (s': i2c_circuit_state) =
-  ^bit_index_ff_tm
+  s' with bit_index := s'.next_bit_index
 End
 
 Definition pend_restart_ff_def:
   pend_restart_ff (fext: i2c_circuit_ext_state) (s: i2c_circuit_state) (s': i2c_circuit_state) =
-  ^pend_restart_ff_tm
+  s' with pend_restart := s'.next_pend_restart
 End
 
 Definition byte_index_ff_def:
   byte_index_ff (fext: i2c_circuit_ext_state) (s: i2c_circuit_state) (s': i2c_circuit_state) =
-  ^byte_index_ff_tm
+  s' with byte_index := s'.next_byte_index
 End
 
 val init_tm = add_x_inits ``
@@ -396,10 +677,46 @@ End
 
 Definition i2c_core_ffs1_def:
   i2c_core_ffs1 = [i2c_core_counter_ff; i2c_core_stretch_idle_cnt_ff; fmt_fifo_rptr_ff;
-                   fmt_fifo_regfile_ff; i2c_core_rx_fifo_wptr_ff; fmt_fifo_wptr_ff; bit_index_ff; pend_restart_ff;
-                   byte_index_ff; i2c_core_rx_fifo_rptr_ff; i2c_core_rx_fifo_regfile; i2c_core_ff]
+                   fmt_fifo_regfile_ff; i2c_core_rx_fifo_wptr_ff; fmt_fifo_wptr_ff; bit_index_ff;
+                   pend_restart_ff; byte_index_ff; i2c_core_rx_fifo_rptr_ff; i2c_core_rx_fifo_regfile;
+                   i2c_core_ff]
 End
 
+(* with dependency taken into account *)        
+Definition i2c_core_combs_def:
+  i2c_core_combs = [
+    fmt_fifo_reset; fmt_fifo_rdata; fmt_fifo_rready; fmt_fifo_empty;
+    fmt_fifo_incr_rptr; fmt_fifo_counter_rptr_wrap;
+    fmt_fifo_counter_rptr_wrap_cnt; fmt_fifo_wvalid; fmt_fifo_full;
+    fmt_fifo_incr_wptr; fmt_fifo_wdata; fmt_fifo_counter_wptr_wrap;
+    fmt_fifo_counter_wptr_wrap_cnt; i2c_core_delay_comb;
+    i2c_core_curr_delay_comb; i2c_core_load_tcount_comb;
+    i2c_core_log_start_comb; i2c_core_log_stop_comb; fmt_fifo_rvalid;
+    fmt_fifo_flag_start_before; fmt_fifo_flag_stop_after;
+    fmt_fifo_flag_read_bytes; fmt_fifo_flag_nak_ok; fmt_byte; req_restart;
+    bit_clr; bit_decr; i2c_core_stretch_en_comb; i2c_core_scl_d_comb;
+    i2c_core_next_scl_rx_val_comb; i2c_core_next_stretch_idle_cnt;
+    i2c_core_next_counter; i2c_core_byte_clr_comb; i2c_core_byte_decr_comb;
+    i2c_core_byte_num_comb; i2c_core_next_byte_index_comb; fifo_depth;
+    counter_gt_one_comb; i2c_core_next_state; i2c_core_read_byte_clr_comb;
+    i2c_core_shift_data_en_comb; i2c_core_next_sda_rx_val_comb;
+    i2c_core_rx_fifo_reset_comb; i2c_core_rx_fifo_rdata_comb;
+    i2c_core_rx_fifo_rready_comb; i2c_core_rx_fifo_empty_comb;
+    i2c_core_rx_fifo_incr_rptr_comb; i2c_core_rx_fifo_counter_rptr_wrap_comb;
+    i2c_core_rx_fifo_counter_rptr_wrap_cnt_comb;
+    i2c_core_rx_fifo_wvalid_comb; i2c_core_rx_fifo_wdata_comb;
+    i2c_core_rx_fifo_full_comb; i2c_core_rx_fifo_incr_wptr_comb;
+    i2c_core_rx_fifo_counter_wptr_wrap_comb;
+    i2c_core_rx_fifo_counter_wptr_wrap_cnt_comb;
+    hw2reg_intr_state_nak_de_comb; next_intr_nak_comb;
+    hw2reg_intr_state_cmd_complete_de_comb;
+    hw2reg_intr_state_cmd_complete_d_comb; next_pend_restart_comb;
+    next_trans_started_comb]                 
+End
+        
+
+(* basis --- successfully generated the deeply embedded *)
+(*
 Definition i2c_core_combs_def:
   i2c_core_combs = [i2c_core_rx_fifo_counter_wptr_wrap_comb; i2c_core_rx_fifo_counter_wptr_wrap_cnt_comb;
                     i2c_core_delay_comb; i2c_core_curr_delay_comb; i2c_core_load_tcount_comb;
@@ -407,20 +724,27 @@ Definition i2c_core_combs_def:
                     i2c_core_next_counter; i2c_core_next_state; fmt_fifo_reset; counter_gt_one_comb;
                     fmt_fifo_rdata; fmt_fifo_rready; fmt_fifo_empty;
                     fmt_fifo_counter_rptr_wrap; fmt_fifo_counter_rptr_wrap_cnt;
-                    fmt_fifo_wvalid; fmt_fifo_full; fmt_fifo_incr_wptr; fmt_fifo_wdata; fmt_fifo_counter_wptr_wrap;
-                    fmt_fifo_counter_wptr_wrap_cnt; i2c_core_log_start_comb; i2c_core_log_stop_comb; fmt_fifo_rvalid;
+                    fmt_fifo_wvalid; fmt_fifo_full; fmt_fifo_incr_wptr; fmt_fifo_wdata;
+                    fmt_fifo_counter_wptr_wrap;
+                    fmt_fifo_counter_wptr_wrap_cnt; i2c_core_log_start_comb; i2c_core_log_stop_comb;
+                    fmt_fifo_rvalid;
                     fmt_fifo_flag_start_before; fmt_fifo_flag_stop_after; fmt_fifo_flag_read_bytes; fmt_byte;
                     req_restart; bit_clr; bit_decr; i2c_core_next_scl_rx_val_comb; i2c_core_byte_clr_comb;
-                    i2c_core_byte_num_comb; i2c_core_next_byte_index_comb; fifo_depth; i2c_core_read_byte_clr_comb;
+                    i2c_core_byte_num_comb; i2c_core_next_byte_index_comb; fifo_depth;
+                    i2c_core_read_byte_clr_comb;
                     i2c_core_shift_data_en_comb; i2c_core_next_sda_rx_val_comb; i2c_core_next_read_byte_comb;
                     i2c_core_rx_fifo_reset_comb; i2c_core_rx_fifo_rdata_comb; i2c_core_rx_fifo_rready_comb;
-                    i2c_core_rx_fifo_empty_comb; i2c_core_rx_fifo_incr_rptr_comb; i2c_core_rx_fifo_counter_rptr_wrap_comb;
-                    i2c_core_rx_fifo_counter_rptr_wrap_cnt_comb; i2c_core_rx_fifo_wvalid_comb; i2c_core_rx_fifo_wdata_comb;
+                    i2c_core_rx_fifo_empty_comb; i2c_core_rx_fifo_incr_rptr_comb;
+                    i2c_core_rx_fifo_counter_rptr_wrap_comb;
+                    i2c_core_rx_fifo_counter_rptr_wrap_cnt_comb; i2c_core_rx_fifo_wvalid_comb;
+                    i2c_core_rx_fifo_wdata_comb;
                     i2c_core_rx_fifo_full_comb; i2c_core_rx_fifo_incr_wptr_comb;
                     hw2reg_intr_state_nak_de_comb; next_intr_nak_comb;
-                    hw2reg_intr_state_cmd_complete_de_comb; hw2reg_intr_state_cmd_complete_d_comb; next_intr_cmd_complete_comb;
+                    hw2reg_intr_state_cmd_complete_de_comb; hw2reg_intr_state_cmd_complete_d_comb;
+                    next_intr_cmd_complete_comb;
                     next_pend_restart_comb; next_trans_started_comb; next_bit_index_comb]
 End
+*)
 
 Definition i2c_circuit_def:
   i2c_circuit = mk_module
@@ -486,7 +810,9 @@ Proof
          i2c_core_rx_fifo_full_comb_def, i2c_core_rx_fifo_incr_wptr_comb_def,
          hw2reg_intr_state_nak_de_comb_def, next_intr_nak_comb_def,
          hw2reg_intr_state_cmd_complete_de_comb_def, hw2reg_intr_state_cmd_complete_d_comb_def, next_intr_cmd_complete_comb_def,
-         next_pend_restart_comb_def, next_trans_started_comb_def, next_bit_index_comb_def]
+         next_pend_restart_comb_def, next_trans_started_comb_def, next_bit_index_comb_def,
+         i2c_core_byte_decr_comb_def, fmt_fifo_flag_nak_ok_def, fmt_fifo_incr_rptr_def
+        ]
 QED
 
 val _ = export_theory ();
