i2c/i2cCircuitCompileScript.sml
@@ -5,17 +5,19 @@ open i2cCircuitTheory;
 
 val _ = new_theory "i2cCircuitCompile";
 
+    (*
 Theorem i2c_circuit_alt_def:
 i2c_circuit =
      mk_module
        (procs
-          ([i2c_core_counter_ff; i2c_core_stretch_idle_cnt_ff;
-            fmt_fifo_rptr_ff; fmt_fifo_regfile_ff; i2c_core_rx_fifo_wptr_ff;
-            fmt_fifo_wptr_ff; bit_index_ff; pend_restart_ff; byte_index_ff;
-            i2c_core_rx_fifo_rptr_ff; i2c_core_rx_fifo_regfile; i2c_core_ff;
-            i2c_reg_top_ff]))
+        ([i2c_core_counter_ff; i2c_core_stretch_idle_cnt_ff;
+          fmt_fifo_rptr_ff; fmt_fifo_regfile_ff; i2c_core_rx_fifo_wptr_ff;
+          fmt_fifo_wptr_ff; bit_index_ff; pend_restart_ff; byte_index_ff;
+          i2c_core_rx_fifo_rptr_ff; i2c_core_rx_fifo_regfile; i2c_core_ff;
+          i2c_reg_top_ff]))
        (procs
-          ([i2c_reg_top_comb_1; i2c_core_rx_fifo_counter_wptr_wrap_comb;
+        ([i2c_reg_top_comb_1;
+          i2c_core_rx_fifo_counter_wptr_wrap_comb;
             i2c_core_rx_fifo_counter_wptr_wrap_cnt_comb; i2c_core_delay_comb;
             i2c_core_curr_delay_comb; i2c_core_load_tcount_comb;
             i2c_core_stretch_en_comb; i2c_core_scl_d_comb;
@@ -50,7 +52,47 @@ i2c_circuit =
 Proof
   rw [i2c_circuit_def, i2c_core_ffs1_def, i2c_core_combs_def]
 QED
+    *)
 
+
+Theorem i2c_circuit_alt_def:
+i2c_circuit =
+     mk_module
+       (procs
+        ([i2c_core_counter_ff; i2c_core_stretch_idle_cnt_ff;
+          fmt_fifo_rptr_ff; fmt_fifo_regfile_ff; i2c_core_rx_fifo_wptr_ff;
+          fmt_fifo_wptr_ff; bit_index_ff; pend_restart_ff; byte_index_ff;
+          i2c_core_rx_fifo_rptr_ff; i2c_core_rx_fifo_regfile; i2c_core_ff;
+          i2c_reg_top_ff]))
+       (procs
+        ([i2c_reg_top_comb_1;
+          next_trans_started_comb; next_pend_restart_comb; hw2reg_intr_state_cmd_complete_d_comb;
+          hw2reg_intr_state_cmd_complete_de_comb; next_intr_nak_comb;
+          hw2reg_intr_state_nak_de_comb; i2c_core_rx_fifo_counter_wptr_wrap_cnt_comb;
+          i2c_core_rx_fifo_counter_wptr_wrap_comb; i2c_core_rx_fifo_incr_wptr_comb;
+          i2c_core_rx_fifo_full_comb; i2c_core_rx_fifo_wdata_comb; i2c_core_rx_fifo_wvalid_comb;
+          i2c_core_rx_fifo_counter_rptr_wrap_cnt_comb; i2c_core_rx_fifo_counter_rptr_wrap_comb;
+          i2c_core_rx_fifo_incr_rptr_comb; i2c_core_rx_fifo_empty_comb; i2c_core_rx_fifo_rready_comb;
+          i2c_core_rx_fifo_rdata_comb; i2c_core_rx_fifo_reset_comb; i2c_core_next_sda_rx_val_comb;
+          i2c_core_shift_data_en_comb; i2c_core_read_byte_clr_comb; i2c_core_next_state;
+          counter_gt_one_comb; fifo_depth; i2c_core_next_byte_index_comb; i2c_core_byte_num_comb;
+          i2c_core_byte_decr_comb; i2c_core_byte_clr_comb; i2c_core_next_counter;
+          i2c_core_next_stretch_idle_cnt; i2c_core_next_scl_rx_val_comb; i2c_core_scl_d_comb;
+          i2c_core_stretch_en_comb; bit_decr; bit_clr; req_restart; fmt_byte;
+          fmt_fifo_flag_nak_ok; fmt_fifo_flag_read_bytes; fmt_fifo_flag_stop_after;
+          fmt_fifo_flag_start_before; fmt_fifo_rvalid; i2c_core_log_stop_comb; i2c_core_log_start_comb;
+          i2c_core_load_tcount_comb; i2c_core_curr_delay_comb; i2c_core_delay_comb;
+          fmt_fifo_counter_wptr_wrap_cnt; fmt_fifo_counter_wptr_wrap; fmt_fifo_wdata;
+          fmt_fifo_incr_wptr; fmt_fifo_full; fmt_fifo_wvalid; fmt_fifo_counter_rptr_wrap_cnt;
+          fmt_fifo_counter_rptr_wrap; fmt_fifo_incr_rptr; fmt_fifo_empty; fmt_fifo_rready;
+          fmt_fifo_rdata; fmt_fifo_reset;
+          i2c_reg_top_comb_2]))
+       i2c_circuit_init
+Proof
+  rw [i2c_circuit_def, i2c_core_ffs1_def, i2c_core_combs_def]
+QED
+    
+    
 local
   val outputs = [
     "reg_rsp_o",
@@ -83,7 +125,7 @@ local
 
 in
   val tstate = init_translator i2c_circuit_alt_def [] comms;
-  val trans_thm = module2hardware tstate i2c_circuit_def [] outputs comms;
+  val trans_thm = module2hardware tstate i2c_circuit_alt_def [] outputs comms;
 end
 
 val verilogstr =
